src/theory/tools/promising/promisingrefinementScript.sml
@@ -1,0 +1,313 @@
+(*
+  Refinement theorems for the promising semantics
+ *)
+
+open HolKernel Parse boolLib bossLib;
+open rich_listTheory arithmeticTheory listTheory pairTheory optionTheory
+     finite_mapTheory relationTheory;
+open bir_programTheory bir_promisingTheory
+     bir_promising_wfTheory bir_programLib
+     promising_thmsTheory refinementTheory;
+
+val _ = new_theory "promisingrefinement";
+
+(* invariants *)
+
+Definition invariant_def:
+  invariant P R = !s s'. P s /\ R s s' ==> P s'
+End
+
+Theorem clstep_preserves_wf_fwdb':
+  !p cid M prom.
+    invariant
+      (λs. (!l. well_formed_fwdb l M (s.bst_coh l) (s.bst_fwdb l)))
+      (λs s'. clstep p cid s M prom s' /\ wf_ext_fwdb p cid s M)
+Proof
+  fs[invariant_def]
+  >> rpt strip_tac
+  >> drule_all clstep_preserves_wf_fwdb
+  >> fs[]
+QED
+
+Theorem parstep_preserves_wf':
+  invariant
+    (λ(cores,M). well_formed_cores cores M /\ well_formed_ext_cores cores)
+    (λ(cores,M) (cores',M'). ?cid. parstep cid cores M cores' M')
+Proof
+  rw[invariant_def,ELIM_UNCURRY]
+  >> drule_all_then assume_tac parstep_preserves_wf
+  >> fs[]
+  >> fs[well_formed_ext_cores_def,parstep_cases]
+  >> rw[wf_ext_p_def,FLOOKUP_UPDATE]
+  >> fs[wf_ext_p_def]
+QED
+
+(* refinement theorems *)
+
+(* inclusion abstract and concrete *)
+Definition state_prog_def:
+  state_prog cores p cores' p' =
+    !cid. IS_SOME $ FLOOKUP cores cid ==>
+            (?s. FLOOKUP cores cid = SOME $ Core cid (BirProgram p) s)
+            /\ ?s'. FLOOKUP cores' cid = SOME $ Core cid (BirProgram p') s'
+End
+
+(* required properties on the refinement relation *)
+Definition rel_prop_def:
+  rel_prop R =
+  !s M s' M' msg.
+    R (s,M) (s',M') ==> s.bst_prom = s'.bst_prom
+      /\ M = M'
+      /\ R
+        (s  with bst_prom updated_by (λx. x ++ [LENGTH M  + 1]), M ++[msg])
+        (s' with bst_prom updated_by (λx. x ++ [LENGTH M' + 1]), M'++[msg])
+End
+
+Theorem rel_prop_imp:
+  rel_prop R ==>
+    !s M s' M'.
+      R (s,M) (s',M') ==> s.bst_prom = s'.bst_prom /\ M = M'
+Proof
+  rw[rel_prop_def]
+  >> first_x_assum drule
+  >> fs[]
+QED
+
+Theorem refinement_RC_clstep_imp_cstep:
+  rel_prop R
+  /\ refinement_RC
+    (λ(s,M) (s',M'). ?prom. clstep (BirProgram p) cid s M prom s' /\ M = M')
+    (λ(s,M) (s',M'). ?prom. clstep (BirProgram p') cid s M prom s' /\ M = M')
+    R
+  ==> refinement_RC
+    (λ(s,M) (s',M'). ?prom. cstep (BirProgram p ) cid s M prom s' M')
+    (λ(s,M) (s',M'). ?prom. cstep (BirProgram p' ) cid s M prom s' M')
+    R
+Proof
+  rpt strip_tac >> rw[refinement_RC_thm,ELIM_UNCURRY]
+  >> dxrule_then strip_assume_tac $ iffLR cstep_cases
+  >~ [`clstep`]
+  >- (
+    gvs[refinement_RC_thm,PULL_EXISTS,ELIM_UNCURRY]
+    >> first_x_assum drule >> fs[]
+    >> disch_then $ dxrule_then assume_tac >> fs[]
+    >> goal_assum $ dxrule_at Any
+    >> dxrule $ SIMP_RULE (srw_ss()) [ELIM_UNCURRY] clstep_imp_cstep_RC
+    >> ho_match_mp_tac RC_MONOTONE
+    >> rw[PULL_EXISTS]
+    >> gvs[]
+    >> goal_assum drule
+  )
+  >> irule_at Any RC_SUBSET
+  >> dsimp[cstep_cases,PULL_EXISTS,ELIM_UNCURRY]
+  >> disj2_tac
+  >> qmatch_asmsub_rename_tac `R cs as`
+  >> PairCases_on `cs` >> PairCases_on `as`
+  >> rename1 `R cs'` >> PairCases_on `cs'`
+  >> gvs[rel_prop_def]
+  >> first_x_assum $ drule_then strip_assume_tac
+  >> gs[FORALL_AND_THM,ELIM_UNCURRY,PULL_EXISTS,EXISTS_PROD]
+  >> irule_at Any EQ_REFL
+  >> fs[]
+QED
+
+Theorem refinement_RTC_clstep_imp_cstep:
+  rel_prop R
+  /\ refinement_RTC
+    (λ(s,M) (s',M'). ?prom. clstep (BirProgram p) cid s M prom s' /\ M = M')
+    (λ(s,M) (s',M'). ?prom. clstep (BirProgram p') cid s M prom s' /\ M = M')
+    R
+  ==> refinement_RTC
+    (λ(s,M) (s',M'). ?prom. cstep (BirProgram p ) cid s M prom s' M')
+    (λ(s,M) (s',M'). ?prom. cstep (BirProgram p' ) cid s M prom s' M')
+    R
+Proof
+  rpt strip_tac >> rw[refinement_RTC_thm,ELIM_UNCURRY]
+  >> dxrule_then strip_assume_tac $ iffLR cstep_cases
+  >~ [`clstep`]
+  >- (
+    gvs[refinement_RTC_thm,PULL_EXISTS,ELIM_UNCURRY]
+    >> first_x_assum drule >> fs[]
+    >> disch_then $ dxrule_then assume_tac >> fs[]
+    >> goal_assum $ dxrule_at Any
+    >> dxrule $ SIMP_RULE (srw_ss()) [ELIM_UNCURRY] clstep_imp_cstep_RTC
+    >> ho_match_mp_tac RTC_MONOTONE
+    >> rw[PULL_EXISTS]
+    >> gvs[]
+    >> goal_assum drule
+  )
+  >> irule_at Any RTC_SINGLE
+  >> dsimp[cstep_cases,PULL_EXISTS,ELIM_UNCURRY]
+  >> disj2_tac
+  >> qmatch_asmsub_rename_tac `R cs as`
+  >> PairCases_on `cs` >> PairCases_on `as`
+  >> rename1 `R cs'` >> PairCases_on `cs'`
+  >> gvs[rel_prop_def]
+  >> first_x_assum $ drule_then strip_assume_tac
+  >> gs[FORALL_AND_THM,ELIM_UNCURRY,PULL_EXISTS,EXISTS_PROD]
+  >> irule_at Any EQ_REFL
+  >> fs[]
+QED
+
+Theorem refinement_RC_clstep_imp_cstep_seq:
+  rel_prop R
+  /\ refinement_RC
+    (λ(s,M) (s',M'). ?prom. clstep (BirProgram p) cid s M prom s' /\ M = M')
+    (λ(s,M) (s',M'). ?prom. clstep (BirProgram p') cid s M prom s' /\ M = M')
+    R
+  ==> refinement_RC
+    (cstep_seq (BirProgram p ) cid)
+    (cstep_seq (BirProgram p') cid)
+    R
+Proof
+  rpt strip_tac >> rw[refinement_RC_thm]
+  >> dxrule_then assume_tac $ iffLR cstep_seq_cases
+  >> gvs[ELIM_UNCURRY,PULL_EXISTS,FORALL_PROD]
+  >> rename1`R (s,M) as` >> PairCases_on `as`
+  (* clstep case *)
+  >- (
+    fs[refinement_RC_thm,PULL_EXISTS,FORALL_PROD]
+    >> first_x_assum $ dxrule_all_then strip_assume_tac
+    >> irule_at Any clstep_imp_cstep_seq_RC
+    >> goal_assum $ dxrule_at Any
+    >> fs[ELIM_UNCURRY]
+  )
+  >~ [`cstep`]
+  >> gvs[cstep_cases]
+  >> qmatch_asmsub_abbrev_tac `clstep _ cid s' M' t s''`
+  >> rename1 `R (s,M) as` >> PairCases_on `as`
+  >> `R (s',M') (as0 with bst_prom updated_by (λx. x ++ t),as1 ++ [msg])` by (
+    dxrule_all_then assume_tac $ iffLR rel_prop_def
+    >> unabbrev_all_tac
+    >> gvs[IMP_CONJ_THM,FORALL_AND_THM]
+  )
+  >> gs[refinement_RC_thm,PULL_EXISTS,LAMBDA_PROD,FORALL_PROD,EXISTS_PROD]
+  >> first_x_assum $ drule_all_then strip_assume_tac
+  >> gvs[ELIM_UNCURRY,RC_DEF]
+  >- (
+    (* contradiction: promise is removed *)
+    unabbrev_all_tac
+    >> imp_res_tac clstep_imp_bst_prom
+    >> dxrule_then imp_res_tac $ rel_prop_imp
+    >> fs[remove_prom_contra,remove_prom_ID]
+  )
+  >> dsimp[cstep_seq_cases,cstep_cases]
+  >> ntac 2 disj2_tac
+  >> unabbrev_all_tac
+  >> goal_assum $ drule_at Any
+  >> imp_res_tac rel_prop_imp
+  >> imp_res_tac clstep_imp_bst_prom
+  >> gvs[EVERY_MEM,IMP_CONJ_THM,remove_prom_ID]
+  >> `~NULL prom` by (
+    spose_not_then assume_tac
+    >> fs[NULL_EQ,remove_prom_ID,remove_prom_contra]
+  )
+  >> qmatch_asmsub_abbrev_tac `remove_prom [t]`
+  >> `!x. MEM x prom ==> x = t` by (
+    spose_not_then assume_tac
+    >> fs[]
+    >> first_x_assum $ drule_then strip_assume_tac
+    >> fs[]
+    >> `MEM x $ remove_prom [t] as0.bst_prom` by
+      simp[remove_prom_def,MEM_FILTER]
+    >> pop_assum mp_tac
+    >> qpat_x_assum `remove_prom _ _ ++ remove_prom _ _ = _` $ rewrite_tac o single o GSYM
+    >> simp[MEM_FILTER,remove_prom_def,COND_RAND,COND_RATOR]
+  )
+  >> `nub prom = [LENGTH M + 1]` by (
+    cheat (* MEM_nub all_distinct_nub *)
+  )
+  >> cheat
+  (* need to add nub function to BSExt for the fulfiled promises prom *)
+  (* need to prove that
+    clstep p cid s M prom s' = clstep p cid s M (nub prom) s'
+  *)
+QED
+
+Theorem refinement_RC_is_certified:
+  rel_prop R
+  /\ refinement_RC
+    (λ(s,M) (s',M'). ?prom. clstep (BirProgram p) cid s M prom s' /\ M = M')
+    (λ(s,M) (s',M'). ?prom. clstep (BirProgram p') cid s M prom s' /\ M = M')
+    R
+  /\ is_certified (BirProgram p) cid cs cM
+  /\ R (cs,cM) (as,aM)
+  ==> is_certified (BirProgram p') cid as aM
+Proof
+  rpt strip_tac >> fs[is_certified_def,cstep_seq_rtc_def]
+  >> drule_all_then assume_tac refinement_RC_clstep_imp_cstep_seq
+  >> dxrule refinement_RC_RTC
+  >> fs[refinement_thm,rel_prop_def]
+  >> disch_then $ dxrule_all_then strip_assume_tac
+  >> qmatch_asmsub_rename_tac `R _ as'` >> PairCases_on `as'`
+  >> goal_assum dxrule
+  >> first_x_assum $ drule_then assume_tac
+  >> fs[]
+QED
+
+Theorem refinement_RC_clstep_imp_parstep:
+  rel_prop R
+  /\ refinement_RC
+      (λ(s,M) (s',M'). ?prom. clstep (BirProgram p) cid s M prom s' /\ M = M')
+      (λ(s,M) (s',M'). ?prom. clstep (BirProgram p') cid s M prom s' /\ M = M')
+      R
+  ==> refinement_RC
+      (λ(cores,M) (cores',M'). parstep cid cores M cores' M')
+      (λ(cores,M) (cores',M'). parstep cid cores M cores' M')
+      (λ(cores,M) (cores',M').
+          state_prog cores p cores' p'
+          /\ !s s'.
+            FLOOKUP cores cid = SOME $ Core cid (BirProgram p) s
+            /\ FLOOKUP cores' cid = SOME $ Core cid (BirProgram p') s'
+            ==> R (s,M) (s',M'))
+Proof
+  rpt strip_tac
+  >> rw[refinement_RC_thm,ELIM_UNCURRY]
+  >> dxrule_then strip_assume_tac $ iffLR parstep_cases
+  >> rename1`SOME $ Core cid p'' s`
+  >> `p'' = BirProgram p` by (
+    fs[state_prog_def,IS_SOME_EXISTS,PULL_EXISTS]
+    >> first_x_assum $ drule_then strip_assume_tac
+    >> gvs[]
+  )
+  >> gvs[]
+  >> drule $ SIMP_RULE(std_ss) [ELIM_UNCURRY] refinement_RC_is_certified
+  >> gvs[PULL_EXISTS,ELIM_UNCURRY]
+  >> disch_then $ drule_then $ drule_then assume_tac
+  (* establish R for post cstep *)
+  >> drule refinement_RC_clstep_imp_cstep
+  >> fs[ELIM_UNCURRY]
+  >> disch_then drule
+  >> simp[refinement_RC_thm,FORALL_PROD,PULL_EXISTS]
+  >> disch_then drule
+  >> `?s. FLOOKUP (FST as) cid = SOME $ Core cid (BirProgram p') s` by
+    fs[state_prog_def]
+  >> first_x_assum $ drule_then assume_tac
+  >> disch_then $ drule_then strip_assume_tac (* abstract step *)
+  >> rename1`R (s', _) as'` >> PairCases_on `as'`
+  >> first_x_assum $ drule_then assume_tac (* is_certified *)
+  (* abstract step cases *)
+  >> dxrule_then assume_tac $ iffLR RC_DEF >> gvs[]
+  (* abstract unchanged *)
+  >- (
+    dsimp[RC_DEF] >> disj1_tac
+    >> conj_tac
+    (* state_prog *)
+    >- (
+      fs[state_prog_def,FLOOKUP_UPDATE] >> rw[] >> fs[]
+    )
+    >> fs[FLOOKUP_UPDATE]
+  )
+  (* change also on abstract level *)
+  >> dsimp[RC_DEF,parstep_cases] >> disj2_tac
+  >> fs[EXISTS_PROD]
+  >> goal_assum drule >> fs[]
+  >> conj_tac
+  (* state_prog *)
+  >- (
+    fs[state_prog_def,FLOOKUP_UPDATE] >> rw[] >> fs[]
+  )
+  >> fs[FLOOKUP_UPDATE]
+QED
+
+val _ = export_theory ();
